\documentclass[crop=false,fleqn]{standalone}
\usepackage{../../../globle-preamble}

\begin{document}
    \textbf{Find $\frac{f(a+h)-f(a)}{h}$ and simplify, where $f(x)=x^3+2x^2-1 x$}

    \begin{align*}
        f(a+h) &= (a+h)^3+2(a+h)^2-1 \\
            &= a^3+h^3+3a^2h+3ah^2+2(a+h)^2 -1 \tag{$\because(a+b)^3=a^3+b^3+3a^2b+3ab^2$} \\
            &= a^3+h^3+3a^2h+3ah^2+2(a^2+2ah+h^2) -1 \\
            &= a^3+h^3+3a^2h+3ah^2+2a^2+4ah+2h^2 -1 \\
        \\
        f(a) &= a^3+2a^2-1\\
        \\
        \frac{f(a+h)-f(a)}{h} &= \frac{(a^3+h^3+3a^2h+3ah^2+2a^2+4ah+2h^2-1) - (a^3+2a^2-1)}{h} \\
            &= \frac{h^3+3a^2h+2ah^2+4ah+2h^2}{h} \\
            &= h^2+3a^2+3ah+4a+2h \\
            &= h^2+3ah+2h+3a^2+4a \tag{By Rearranging} \\
            &= h^2+(3a+2)h+3a^2+4a
    \end{align*}
\end{document}
