\documentclass[crop=false,fleqn]{standalone}
\usepackage{../../../globle-preamble}

\begin{document}
    \textbf{Find $\frac{f(a+h)-f(a)}{h}$ and simplify, where $f(x)=\sin(x)$}


    \begin{align*}
        f(a+h) &= \sin(a+h) \\
        \\
        f(a) &= \sin(a) \\
        \\
        \frac{f(a+h)-f(a)}{h} &= \frac{\sin(a+h)-\sin(a)}{h} \\
            &= \frac{1}{h} \times 2
                \cos\left(\frac{a + h + a}{2}\right)
                \sin\left(\frac{a + h - a}{2}\right)
                \tag{$ \because \sin(p)-\sin(q) =
                    2 \cos\left(\frac{p+q}{2}\right)
                    \sin\left(\frac{p-q}{2}\right)
                $} \\
            &= \frac{2}{h}
                \cos\left(\frac{2a+h}{2}\right)
                \sin\left(\frac{h}{2}\right)
    \end{align*}
\end{document}
