\documentclass[crop=false,fleqn]{standalone}
\usepackage{../../../globle-preamble}

\begin{document}
    \subsubsection{Question 5}
    \textbf{Given $f(x)=x^3-ax^2+bx+1$. If $f(2)=-3$ and $f(-1)=0$, find the values of $a$ and $b$}

    \begin{align*}
        f(x) &= x^3 - ax^2 + bx + 1 \tag{1}
    \end{align*}

    Putting $x = 2$ in equation (1)
    \begin{align*}
        f(2) &= 2^3 - a(2)^2 + 2b + 1 \\
            &= 8 - 4a + 2b + 1 \\
            &= 9 - 4a + 2b \\
        \\
        \implies -3 &= 9 - 4a + 2b \tag{As $f(2) = -3$} \\
            -4a + 2b &= -3 -9 \tag{By Rearranging} \\
            -2(2a - b) &= -12 \\
            2a - b &= 6 \tag{2}
    \end{align*}



    Putting $x = -1$ in equation (1)
    \begin{align*}
        f(-1) &= -1^3 - a(-1)^2 - 1b + 1 \\
            &= -1 - a - b + 1 \\
            &= -a -b \\
        \\
        \implies 0 &= -a -b \tag{As $f(-1) = 0$} \\
            a &= -b \tag{3} \\
    \end{align*}

    Putting $a = -b$ in equation (2)
    \begin{align*}
        2(-b) -b &= 6 \\
        -3b &= 6 \\
        b &= \frac{6}{-3} \\
        b &= -2
    \end{align*}

    Putting $b = -2$ in equation (3)
    \begin{align*}
        a &= - (-2) \\
        a &= 2
    \end{align*}

    Thus $a=2$ and $b=-2$.
\end{document}
